Implement direction in tree definitions and interpretation

warblreequiv/TreeMSInterp.v
@@ -16,13 +16,13 @@ Definition reset_groups_ms {F H} `{CharacterMarker H} `{Result.AssertionError F}
   end in
   (match_state inp endInd cap').
 
-(* A list of currently open groups, with for each of them their ID and the position at which they were opened.
+(* A list of currently open groups, with for each of them their ID, the position at which they were opened and the group's direction.
    This is needed because we want to be able to express the result of the first branch of a sub-backtracking tree,
    which can close groups that are not opened within this tree and whose opening indices the Matchers and TMatchers
    do not record in the MatchStates passed to subsequent calls.
    *An extended match state is a MatchState with a list of open groups with indices.* It allows to model the capture
    of group opening indices in continuations. *)
-Definition open_groups := list (Groups.group_id * integer).
+Definition open_groups := list (Groups.group_id * integer * Direction).
 
 
 (* Close group id opened in gl at index end_index. If group id was indeed open, returns the new list of open groups
@@ -31,22 +31,24 @@ Definition open_groups := list (Groups.group_id * integer).
 Fixpoint close_group (id: Groups.group_id) (gl: open_groups) end_index: CaptureRange * open_groups :=
   match gl with
   | nil => (capture_range (-1)%Z (-1)%Z, nil)
-  | (id', start)::q =>
-    if id == id' then
+  | (id', ind, dir)::q =>
+      if id == id' then
+        let start := match dir with forward => ind | backward => end_index end in
+        let groupEnd := match dir with forward => end_index | backward => ind end in
       (capture_range start end_index, q)
     else
       let (range, q') := close_group id q end_index in
-      (range, (id', start)::q')
+      (range, (id', ind, dir)::q')
   end.
 
 (* TODO Direction *)
 (* Apply the given group action to the extended match state composed of a MatchState and a list of open groups with
    opening indices.
    If we try to close a nonexisting group or clear nonexisting capture ranges, do nothing. *)
-Definition group_effect' {F H} `{CharacterMarker H} `{Result.AssertionError F} (g: groupaction) (s: MatchState) (gl: open_groups): MatchState * open_groups :=
+Definition group_effect' {F H} `{CharacterMarker H} `{Result.AssertionError F} (g: groupaction) (s: MatchState) (gl: open_groups) (dir: Direction) : MatchState * open_groups :=
   match g with
   | Open gid =>
-      (s, (gid, MatchState.endIndex s)::gl)
+      (s, (gid, MatchState.endIndex s, dir)::gl)
   | Close gid =>
       let cap := MatchState.captures s in
       let (range, gl') := close_group gid gl (MatchState.endIndex s) in
@@ -68,35 +70,35 @@ Definition group_effect' {F H} `{CharacterMarker H} `{Result.AssertionError F} (
 (* TODO Direction *)
 (* Given a sub-backtracking tree and an extended match state, retrieve the highest priority result represented
    by the subtree. *)
-Fixpoint tree_res' {F} `{Result.AssertionError F} (t:tree) (s: MatchState) (gl: open_groups): option MatchState :=
+Fixpoint tree_res' {F} `{Result.AssertionError F} (t:tree) (s: MatchState) (gl: open_groups) (dir: Direction): option MatchState :=
   match t with
   | Mismatch => None
   | Match => Some s
   | Choice t1 t2 =>
-      let res1 := tree_res' t1 s gl in
+      let res1 := tree_res' t1 s gl dir in
       match res1 with
-      | None => tree_res' t2 s gl
+      | None => tree_res' t2 s gl dir
       | Some _ => res1
       end
   | Read c t1 =>
-    tree_res' t1 (advance_ms s) gl
+    tree_res' t1 (advance_ms s dir) gl dir
   | CheckFail _ => None
-  | CheckPass _ t1 => tree_res' t1 s gl
+  | CheckPass _ t1 => tree_res' t1 s gl dir
   | GroupAction g t1 => 
-      let (s', gl') := group_effect' g s gl in tree_res' t1 s' gl'
+      let (s', gl') := group_effect' g s gl dir in tree_res' t1 s' gl' dir
   | LK lk tlk t =>
       match positivity lk with
       | true =>
-          match tree_res' tlk s nil with (* Contrary to the original tree_res, and to respect the ECMA semantics, we use the empty open group list instead of the original one. In practical situations, this does not change anything as tlk cannot close any group that it itself does not open, but now we don't have to prove it. *)
+          match tree_res' tlk s nil (lk_dir lk) with (* Contrary to the original tree_res, and to respect the ECMA semantics, we use the empty open group list instead of the original one. In practical situations, this does not change anything as tlk cannot close any group that it itself does not open, but now we don't have to prove it. *)
           | Some mslk =>
               (* using the captures defined in the first branch of the lookahead; the open groups remain unchanged because the lookaround is well-parenthesized *)
-              tree_res' t (match_state (MatchState.input s) (MatchState.endIndex s) (MatchState.captures mslk)) gl
+              tree_res' t (match_state (MatchState.input s) (MatchState.endIndex s) (MatchState.captures mslk)) gl dir
           | None => None (* unreachable in valid trees *)
           end
-      | false => match tree_res' tlk s nil with (* Same here *)
+      | false => match tree_res' tlk s nil (lk_dir lk) with (* Same here *)
           (* using previous captures *)
           | Some _ => None (* unreachable in valid trees *)
-          | None => tree_res' t s gl
+          | None => tree_res' t s gl dir
           end
       end
   | LKFail _ _ => None
@@ -107,13 +109,13 @@ Fixpoint tree_res' {F} `{Result.AssertionError F} (t:tree) (s: MatchState) (gl: 
 Definition first_branch' {F} `{Result.AssertionError F} (t: tree) :=
   let dummystr := [] in
   let cap := List.repeat undefined (1 + max_gid_tree t) in
-  tree_res' t (match_state dummystr 0%Z cap) [].
+  tree_res' t (match_state dummystr 0%Z cap) [] forward.
 
 
 (** * Independence of presence or absence of result from the MatchState and open groups *)
 Lemma result_indep_gm {F} `{Result.AssertionError F}:
-  forall t ms1 gl1 ms2 gl2,
-    tree_res' t ms1 gl1 = None -> tree_res' t ms2 gl2 = None.
+  forall t dir ms1 gl1 ms2 gl2,
+    tree_res' t ms1 gl1 dir = None -> tree_res' t ms2 gl2 dir = None.
 Proof.
   intro t. induction t; eauto.
   - discriminate.
